<?xml version="1.0"?>

<!DOCTYPE rdf:RDF [
    <!ENTITY bio "http://purl.bioontology.org/" >
    <!ENTITY owl "http://www.w3.org/2002/07/owl#" >
    <!ENTITY obo "http://purl.obolibrary.org/obo/" >
    <!ENTITY dc "http://purl.org/dc/elements/1.1/" >
    <!ENTITY xsd "http://www.w3.org/2001/XMLSchema#" >
    <!ENTITY rdfs "http://www.w3.org/2000/01/rdf-schema#" >
    <!ENTITY rdf "http://www.w3.org/1999/02/22-rdf-syntax-ns#" >
    <!ENTITY oboInOwl "http://www.geneontology.org/formats/oboInOwl#" >
]>

<rdf:RDF xmlns="&obo;ontoneo/import/omiabis_import.owl#"
     xml:base="&obo;ontoneo/import/omiabis_import.owl"
     xmlns:dc="http://purl.org/dc/elements/1.1/"
     xmlns:obo="http://purl.obolibrary.org/obo/"
     xmlns:rdfs="http://www.w3.org/2000/01/rdf-schema#"
     xmlns:foaf="http://xmlns.com/foaf/0.1/"
     xmlns:owl="http://www.w3.org/2002/07/owl#"
     xmlns:xsd="http://www.w3.org/2001/XMLSchema#"
     xmlns:rdf="http://www.w3.org/1999/02/22-rdf-syntax-ns#">
    <owl:Ontology rdf:about="&obo;ontoneo/import/omiabis_import.owl">
        <dc:title xml:lang="en">Ontologized MIABIS</dc:title>
        <rdfs:comment xml:lang="en">PERSON: Fernanda Farinelli
This owl file represents the necessary entities of OMIABIS that are reused in OntONeo Ontology. This file was created using Ontofox and some intermediary entities were not imported.</rdfs:comment>
        <rdfs:comment xml:lang="en">OMIABIS subset applied to OntONeo ontology.</rdfs:comment>
        <owl:versionIRI rdf:resource="&obo;ontoneo/import/omiabis_import.owl"/>
    </owl:Ontology>
	
    


    <!-- 
    ///////////////////////////////////////////////////////////////////////////////////////
    //
    // Classes
    //
    ///////////////////////////////////////////////////////////////////////////////////////
     -->
	 
    <!-- http://purl.obolibrary.org/obo/OMIABIS_0000021 -->

    <owl:Class rdf:about="http://purl.obolibrary.org/obo/OMIABIS_0000021">
        <rdfs:label xml:lang="en">telephone number</rdfs:label>
        <rdfs:subClassOf rdf:resource="http://purl.obolibrary.org/obo/IAO_0000300"/>
        <rdfs:subClassOf>
            <owl:Restriction>
                <owl:onProperty rdf:resource="http://purl.obolibrary.org/obo/BFO_0000051"/>
                <owl:allValuesFrom rdf:resource="http://purl.obolibrary.org/obo/IAO_0000029"/>
            </owl:Restriction>
        </rdfs:subClassOf>
        <obo:IAO_0000117>Mathias Brochhausen</obo:IAO_0000117>
        <obo:IAO_0000115 xml:lang="en">A telephone number  is a textual entity consisting of a sequence of digits used to call from one telephone line to another in a public switched telephone network.</obo:IAO_0000115>
        <rdfs:comment xml:lang="en">MB: This class should probably be a subclass to CRID. However, the textual definition of CRID right now states that each instance has the CRID identifier as a part. This is not the case for telephone numbers. Therefore, they cannot be subsumed under CRID now. I am looking into changing IAO accordingly. Once that is done, the class ought to be a subclass of CRID.</rdfs:comment>
        <obo:IAO_0000119>http://en.wikipedia.org/wiki/Telephone_number</obo:IAO_0000119>
    </owl:Class>
</rdf:RDF>	
	